proofs/serialize/B: panic freedom (modulo `decompress_pre`)

proofs/fstar/extraction-edited/Libcrux.Kem.Kyber.Serialize.PartB.fst
@@ -5,9 +5,46 @@ open FStar.Mul
 open MkSeq
 open Libcrux.Kem.Kyber.Serialize.PartA
 
-#push-options "--fuel 0 --ifuel 1 --z3rlimit 100"
+let cast_bound_lemma 
+  #t #u
+  (n: int_t t) 
+  (d: bit_num t)
+  : Lemma (requires bounded n d /\ d <= bits u /\ unsigned u /\ v n >= 0)
+          (ensures  bounded (cast #(int_t t) #(int_t u) n) d)
+          [SMTPat (bounded n d); SMTPat (cast #(int_t t) #(int_t u) n)]
+  = ()
+assume val lemma_get_bit_bounded' #t (x:int_t t) (d:bit_num t):
+  Lemma (requires forall i. v i > d ==> get_bit x i == 0)
+        (ensures bounded x d)
+assume val intro_refinement_slice #p (a: t_Slice 't {forall i. p (Seq.index a i)})
+  : r: t_Slice (x: 't {p x}) {Seq.length r == Seq.length a /\ (forall i. Seq.index a i == Seq.index r i)}
+  = admit ()
+assume val elim_refinement_slice #p (a: t_Slice (x: 't {p x}))
+  : r: t_Slice 't {(forall i. p (Seq.index r i)) /\ Seq.length r == Seq.length a /\ (forall i. Seq.index a i == Seq.index r i)}
+  = admit ()
+#push-options "--z3rlimit 60"
+let int_t_d_cast_lemma #t #u d (n: int_t_d t d)
+  : Lemma (requires bits t < bits u /\ v n >= 0)
+          (ensures bounded (cast #(int_t t) #(int_t u) n) d)
+          [SMTPat (bounded (cast #(int_t t) #(int_t u) n) d)]
+  = Math.Lemmas.pow2_double_mult (bits u - 1);
+    Math.Lemmas.small_mod (v n) (modulus u)
+let mul_in_range (n m: nat)
+  : Lemma
+    (requires n <= 256 /\ m <= 256)
+    (ensures range (n * m) usize_inttype)
+  = Math.Lemmas.pow2_plus 8 8;
+    Math.Lemmas.pow2_le_compat 32 16
+#pop-options
+
+
+
+
+
+
+#push-options "--fuel 0 --ifuel 1 --query_stats --z3rlimit 100"
 let compress_then_serialize_10_
-      (v_OUT_LEN: usize)
+      v_OUT_LEN
       re
     =
   let accT = t_Array u8 v_OUT_LEN in
@@ -31,16 +68,15 @@ let compress_then_serialize_10_
     //   )
     True
   in
-  admit ();
   let serialized:t_Array u8 v_OUT_LEN = Rust_primitives.Hax.repeat 0uy v_OUT_LEN in
   let serialized:t_Array u8 v_OUT_LEN =
-    Rust_primitives.Iterators.foldi_chunks_exact #i32 #accT #inv
-      (Rust_primitives.unsize re.Libcrux.Kem.Kyber.Arithmetic.f_coefficients <: t_Slice i32)
+    Rust_primitives.Iterators.foldi_chunks_exact #_ #accT #inv
+      (re.Libcrux.Kem.Kyber.Arithmetic.f_coefficients)
       (sz 4)
       (serialized)
       (fun serialized temp_1_ ->
           let serialized:t_Array u8 v_OUT_LEN = serialized in
-          let i, coefficients:(usize & t_Slice i32) = temp_1_ in
+          let i, coefficients:(usize & _) = temp_1_ in
           let coefficient1:i32 =
             Libcrux.Kem.Kyber.Compress.compress_ciphertext_coefficient 10uy
               (Libcrux.Kem.Kyber.Arithmetic.to_unsigned_representative (coefficients.[ sz 0 ] <: i32
@@ -106,7 +142,7 @@ let compress_then_serialize_10_
 let update5
   #n
   (s: t_Array 't n)
-  (offset: usize {v offset + 5 <= Seq.length s})
+  (offset: usize {v offset + 5 <= v n})
   (i0 i1 i2 i3 i4: 't)
   : s': t_Array 't n {
      Seq.index s' (v offset +  0) == i0  /\
@@ -123,48 +159,21 @@ let update5
     let s = update_at_usize s (offset +! sz  3) i3  in
     let s = update_at_usize s (offset +! sz  4) i4  in
     s
-
-let update11 
-  #n
-  (s: t_Array 't n)
-  (offset: usize {v offset + 11 <= Seq.length s})
-  (i0 i1 i2 i3 i4 i5 i6 i7 i8 i9 i10: 't)
-  : s': t_Array 't n {
-     Seq.index s' (v offset +  0) == i0  /\
-     Seq.index s' (v offset +  1) == i1  /\
-     Seq.index s' (v offset +  2) == i2  /\
-     Seq.index s' (v offset +  3) == i3  /\
-     Seq.index s' (v offset +  4) == i4  /\
-     Seq.index s' (v offset +  5) == i5  /\
-     Seq.index s' (v offset +  6) == i6  /\
-     Seq.index s' (v offset +  7) == i7  /\
-     Seq.index s' (v offset +  8) == i8  /\
-     Seq.index s' (v offset +  9) == i9  /\
-     Seq.index s' (v offset + 10) == i10 /\
-     (forall i. (i < v offset \/ i >= v offset + 11) ==> Seq.index s' i == Seq.index s i)
-    }
-  = let open Rust_primitives.Hax.Monomorphized_update_at in
-    let s = update5 s offset i0 i1 i2 i3 i4 in
-    let s = update5 s (offset +! sz 5) i5 i6 i7 i8 i9 in
-    let s = update_at_usize s (offset +! sz 10) i10 in
-    s
 #pop-options
 
-#push-options "--fuel 0 --ifuel 1 --z3rlimit 100"
+#push-options "--fuel 0 --ifuel 1 --z3rlimit 100 --query_stats --split_queries no"
 let compress_then_serialize_11_
       v_OUT_LEN re
   =
   let inv = fun (acc: t_Array u8 v_OUT_LEN) (i: usize) -> True in
   let serialized:t_Array u8 v_OUT_LEN = Rust_primitives.Hax.repeat 0uy v_OUT_LEN in
-  admit();
   let serialized:t_Array u8 v_OUT_LEN =
     Rust_primitives.Iterators.foldi_chunks_exact #_ #_ #inv
-      (Rust_primitives.unsize re.Libcrux.Kem.Kyber.Arithmetic.f_coefficients <: t_Slice i32)
+      (Rust_primitives.unsize re.Libcrux.Kem.Kyber.Arithmetic.f_coefficients)
       (sz 8)
       serialized
       (fun serialized temp_1_ ->
           let serialized:t_Array u8 v_OUT_LEN = serialized in
-          admit();
           let i, coefficients:(usize & t_Array Libcrux.Kem.Kyber.Arithmetic.wfFieldElement (sz 8)) = temp_1_ in
           let coefficient1 =
             Libcrux.Kem.Kyber.Compress.compress_ciphertext_coefficient 11uy
@@ -241,22 +250,69 @@ let compress_then_serialize_11_
               coefficient7
               coefficient8
           in
-          assume (11 * v i + 11 <= v v_OUT_LEN);
-          let serialized = 
-            update11 serialized (sz 11 *! i) 
-              coef1 coef2 coef3 coef4 coef5 coef6 coef7 coef8 coef9 coef10 coef11
+          assert_spinoff (v i < 32 ==> 11 * v i + 11 <= 32 * 11);
+          assert_spinoff (v i < 32 ==> range (v (sz 11) * v i) usize_inttype);
+          let serialized:t_Array u8 v_OUT_LEN =
+            Rust_primitives.Hax.Monomorphized_update_at.update_at_usize serialized
+              (sz 11 *! i <: usize)
+              coef1
+          in
+          let serialized:t_Array u8 v_OUT_LEN =
+            Rust_primitives.Hax.Monomorphized_update_at.update_at_usize serialized
+              ((sz 11 *! i <: usize) +! sz 1 <: usize)
+              coef2
+          in
+          let serialized:t_Array u8 v_OUT_LEN =
+            Rust_primitives.Hax.Monomorphized_update_at.update_at_usize serialized
+              ((sz 11 *! i <: usize) +! sz 2 <: usize)
+              coef3
+          in
+          let serialized:t_Array u8 v_OUT_LEN =
+            Rust_primitives.Hax.Monomorphized_update_at.update_at_usize serialized
+              ((sz 11 *! i <: usize) +! sz 3 <: usize)
+              coef4
+          in
+          let serialized:t_Array u8 v_OUT_LEN =
+            Rust_primitives.Hax.Monomorphized_update_at.update_at_usize serialized
+              ((sz 11 *! i <: usize) +! sz 4 <: usize)
+              coef5
+          in
+          let serialized:t_Array u8 v_OUT_LEN =
+            Rust_primitives.Hax.Monomorphized_update_at.update_at_usize serialized
+              ((sz 11 *! i <: usize) +! sz 5 <: usize)
+              coef6
+          in
+          let serialized:t_Array u8 v_OUT_LEN =
+            Rust_primitives.Hax.Monomorphized_update_at.update_at_usize serialized
+              ((sz 11 *! i <: usize) +! sz 6 <: usize)
+              coef7
+          in
+          let serialized:t_Array u8 v_OUT_LEN =
+            Rust_primitives.Hax.Monomorphized_update_at.update_at_usize serialized
+              ((sz 11 *! i <: usize) +! sz 7 <: usize)
+              coef8
+          in
+          let serialized:t_Array u8 v_OUT_LEN =
+            Rust_primitives.Hax.Monomorphized_update_at.update_at_usize serialized
+              ((sz 11 *! i <: usize) +! sz 8 <: usize)
+              coef9
+          in
+          let serialized:t_Array u8 v_OUT_LEN =
+            Rust_primitives.Hax.Monomorphized_update_at.update_at_usize serialized
+              ((sz 11 *! i <: usize) +! sz 9 <: usize)
+              coef10
+          in
+          let serialized:t_Array u8 v_OUT_LEN =
+            Rust_primitives.Hax.Monomorphized_update_at.update_at_usize serialized
+              ((sz 11 *! i <: usize) +! sz 10 <: usize)
+              coef11
           in
           serialized)
   in
   serialized
 #pop-options
 
-
-
-let compress_then_serialize_4_
-      (v_OUT_LEN: usize)
-      (re: Libcrux.Kem.Kyber.Arithmetic.wfPolynomialRingElement)
-    : t_Array u8 v_OUT_LEN =
+let compress_then_serialize_4_ v_OUT_LEN re =
   let serialized:t_Array u8 v_OUT_LEN = Rust_primitives.Hax.repeat 0uy v_OUT_LEN in
   let accT = t_Array u8 v_OUT_LEN in
   let inv (acc: accT) (i: usize) = True in
@@ -267,7 +323,6 @@ let compress_then_serialize_4_
       serialized
       (fun serialized temp_1_ ->
           let serialized:t_Array u8 v_OUT_LEN = serialized in
-          admit();
           let i, coefficients:(usize & t_Array Libcrux.Kem.Kyber.Arithmetic.wfFieldElement (sz 2)) = temp_1_ in
           let coefficient1:u8 =
             cast (Libcrux.Kem.Kyber.Compress.compress_ciphertext_coefficient 4uy
@@ -293,7 +348,6 @@ let compress_then_serialize_4_
             <:
             u8
           in
-          assume (i <. v_OUT_LEN);
           let serialized:t_Array u8 v_OUT_LEN =
             Rust_primitives.Hax.Monomorphized_update_at.update_at_usize serialized
               i
@@ -304,22 +358,20 @@ let compress_then_serialize_4_
   serialized
 
 let compress_then_serialize_5_
-      (v_OUT_LEN: usize)
-      (re: Libcrux.Kem.Kyber.Arithmetic.wfPolynomialRingElement)
-    : t_Array u8 v_OUT_LEN =
+      v_OUT_LEN
+      re
+  =
   let serialized:t_Array u8 v_OUT_LEN = Rust_primitives.Hax.repeat 0uy v_OUT_LEN in
   let accT = t_Array u8 v_OUT_LEN in
   let inv (acc: accT) (i: usize) = True in
-  admit();
   let serialized:t_Array u8 v_OUT_LEN =
     Rust_primitives.Iterators.foldi_chunks_exact #_ #_ #inv
       (Rust_primitives.unsize re.Libcrux.Kem.Kyber.Arithmetic.f_coefficients)
       (sz 8)
       serialized
       (fun serialized temp_1_ ->
-          admit ();
           let serialized:t_Array u8 v_OUT_LEN = serialized in
-          let i, coefficients:(usize & t_Array i32 (sz 8)) = temp_1_ in
+          let i, coefficients:(usize & t_Array Libcrux.Kem.Kyber.Arithmetic.wfFieldElement (sz 8)) = temp_1_ in
           let coefficient1:u8 =
             cast (Libcrux.Kem.Kyber.Compress.compress_ciphertext_coefficient 5uy
                   (Libcrux.Kem.Kyber.Arithmetic.to_unsigned_representative (coefficients.[ sz 0 ]
@@ -404,6 +456,14 @@ let compress_then_serialize_5_
             <:
             u8
           in
+          let coefficient8' = Libcrux.Kem.Kyber.Compress.compress_ciphertext_coefficient 5uy
+                  (Libcrux.Kem.Kyber.Arithmetic.to_unsigned_representative (coefficients.[ sz 7 ]
+                        <:
+                        i32)
+                    <:
+                    u16)
+                <:
+                i32 in
           let coefficient8:u8 =
             cast (Libcrux.Kem.Kyber.Compress.compress_ciphertext_coefficient 5uy
                   (Libcrux.Kem.Kyber.Arithmetic.to_unsigned_representative (coefficients.[ sz 7 ]
@@ -426,6 +486,8 @@ let compress_then_serialize_5_
               coefficient6
               coefficient8
           in
+          assert_spinoff (v i < 32 ==> 5 * v i + 5 <= 32 * 5);
+          assert_spinoff (v i < 32 ==> range (v (sz 5) * v i) usize_inttype);
           let serialized:t_Array u8 v_OUT_LEN =
             Rust_primitives.Hax.Monomorphized_update_at.update_at_usize serialized
               (sz 5 *! i <: usize)
@@ -455,26 +517,24 @@ let compress_then_serialize_5_
   in
   serialized
 
-let compress_then_serialize_message (re: Libcrux.Kem.Kyber.Arithmetic.wfPolynomialRingElement) =
+let compress_then_serialize_message re =
   let serialized:t_Array u8 (sz 32) = Rust_primitives.Hax.repeat 0uy (sz 32) in
   let accT = t_Array u8 (sz 32) in
   let inv (acc: accT) (i: usize) = True in
-  admit();
   let serialized:t_Array u8 (sz 32) =
     Rust_primitives.Iterators.foldi_chunks_exact #_ #_ #inv
-      (Rust_primitives.unsize re.Libcrux.Kem.Kyber.Arithmetic.f_coefficients)
+      (re.Libcrux.Kem.Kyber.Arithmetic.f_coefficients)
       (sz 8)
       serialized
       (fun serialized temp_1_ ->
-          admit ();
           let serialized:t_Array u8 (sz 32) = serialized in
-          let i, coefficients:(usize & t_Slice i32) = temp_1_ in
+          let i, coefficients:(usize & t_Array Libcrux.Kem.Kyber.Arithmetic.wfFieldElement _) = temp_1_ in
           Rust_primitives.Iterators.foldi_slice #_ #_ #(fun _ _ -> True) 
             coefficients
             serialized
             (fun serialized temp_1_ ->
                 let serialized:t_Array u8 (sz 32) = serialized in
-                let j, coefficient:(usize & i32) = temp_1_ in
+                let j, coefficient:(usize & Libcrux.Kem.Kyber.Arithmetic.wfFieldElement) = temp_1_ in
                 let coefficient:u16 =
                   Libcrux.Kem.Kyber.Arithmetic.to_unsigned_representative coefficient
                 in
@@ -487,21 +547,29 @@ let compress_then_serialize_message (re: Libcrux.Kem.Kyber.Arithmetic.wfPolynomi
           <:
           t_Array u8 (sz 32))
   in
-  admit ();
+  admit (); // P-F 
   serialized
 
 let compress_then_serialize_ring_element_u #p
-      (v_COMPRESSION_FACTOR v_OUT_LEN: usize)
+      (v_COMPRESSION_FACTOR: usize) 
+      (v_OUT_LEN: usize {
+        match v v_COMPRESSION_FACTOR with
+        | 10 -> v v_OUT_LEN >= 320
+        | 11 -> v v_OUT_LEN >= 352
+        | _ -> False
+      })
       (re: Libcrux.Kem.Kyber.Arithmetic.wfPolynomialRingElement) =
   let _:Prims.unit = () <: Prims.unit in
+  assert (
+    (v (cast (v_COMPRESSION_FACTOR <: usize) <: u32) == 11) \/
+    (v (cast (v_COMPRESSION_FACTOR <: usize) <: u32) == 10)
+  );
   Rust_primitives.Integers.mk_int_equiv_lemma #usize_inttype (v v_COMPRESSION_FACTOR);
-  admit ();
   match cast (v_COMPRESSION_FACTOR <: usize) <: u32 with
   | 10ul -> compress_then_serialize_10_ v_OUT_LEN re
   | 11ul -> compress_then_serialize_11_ v_OUT_LEN re
   | _ ->
     Rust_primitives.Hax.never_to_any (Core.Panicking.panic "internal error: entered unreachable code"
-
         <:
         Rust_primitives.Hax.t_Never)
 
@@ -509,7 +577,10 @@ let compress_then_serialize_ring_element_v #p v_COMPRESSION_FACTOR v_OUT_LEN re 
   let _:Prims.unit = () <: Prims.unit in
   Rust_primitives.Integers.mk_int_equiv_lemma #usize_inttype (v v_COMPRESSION_FACTOR);
   let res = 
-  admit ();
+  assert (
+    (v (cast (v_COMPRESSION_FACTOR <: usize) <: u32) == 4) \/
+    (v (cast (v_COMPRESSION_FACTOR <: usize) <: u32) == 5)
+  );
   match cast (v_COMPRESSION_FACTOR <: usize) <: u32 with
   | 4ul -> compress_then_serialize_4_ v_OUT_LEN re
   | 5ul -> compress_then_serialize_5_ v_OUT_LEN re
@@ -519,12 +590,19 @@ let compress_then_serialize_ring_element_v #p v_COMPRESSION_FACTOR v_OUT_LEN re 
         <:
         Rust_primitives.Hax.t_Never)
   in
-  admit(); //P-F
+  admit (); // P-F
   res
 
-#push-options "--z3rlimit 150"
-let deserialize_then_decompress_10_ (serialized: t_Slice u8)
-    =
+let decompress_coefficients_10_ (byte2 byte1 byte3 byte4 byte5: int_t_d i32_inttype 8)
+    : (tuple: (i32 & i32 & i32 & i32) {
+          int_arr_bitwise_eq
+                (create5 (byte1, byte2, byte3, byte4, byte5)) 8
+                (create4 tuple) 10
+      })
+    = decompress_coefficients_10_ byte2 byte1 byte3 byte4 byte5
+
+#push-options "--z3rlimit 60"
+let deserialize_then_decompress_10_ serialized =
   let _:Prims.unit = () <: Prims.unit in
   let re:Libcrux.Kem.Kyber.Arithmetic.wfPolynomialRingElement =
     Libcrux.Kem.Kyber.Arithmetic.cast_poly_b Libcrux.Kem.Kyber.Arithmetic.impl__PolynomialRingElement__ZERO
@@ -539,102 +617,91 @@ let deserialize_then_decompress_10_ (serialized: t_Slice u8)
       (fun re temp_1_ ->
           let re:Libcrux.Kem.Kyber.Arithmetic.wfPolynomialRingElement = re in
           let i, bytes:(usize & t_Array u8 (sz 5)) = temp_1_ in
-          assume (length bytes == sz 5);
-          let byte1:i32 = cast (bytes.[ sz 0 ] <: u8) <: i32 in
-          let byte2:i32 = cast (bytes.[ sz 1 ] <: u8) <: i32 in
-          let byte3:i32 = cast (bytes.[ sz 2 ] <: u8) <: i32 in
-          let byte4:i32 = cast (bytes.[ sz 3 ] <: u8) <: i32 in
-          let byte5:i32 = cast (bytes.[ sz 4 ] <: u8) <: i32 in
-          (*
-          assume (int_t_has_bit_num byte1 8);
-          assume (int_t_has_bit_num byte2 8);
-          assume (int_t_has_bit_num byte3 8);
-          assume (int_t_has_bit_num byte4 8);
-          assume (int_t_has_bit_num byte5 8); *)
-          admit ();
-          let coefficient1, coefficient2, coefficient3, coefficient4:(i32 & i32 & i32 & i32) =
+          let byte1: int_t_d i32_inttype 8 = cast (bytes.[ sz 0 ] <: u8) <: i32 in
+          let byte2: int_t_d i32_inttype 8 = cast (bytes.[ sz 1 ] <: u8) <: i32 in
+          let byte3: int_t_d i32_inttype 8 = cast (bytes.[ sz 2 ] <: u8) <: i32 in
+          let byte4: int_t_d i32_inttype 8 = cast (bytes.[ sz 3 ] <: u8) <: i32 in
+          let byte5: int_t_d i32_inttype 8 = cast (bytes.[ sz 4 ] <: u8) <: i32 in
+          let coefficient1, coefficient2, coefficient3, coefficient4 =
             decompress_coefficients_10_ byte2 byte1 byte3 byte4 byte5
           in
-          admit ();
           assume (Libcrux.Kem.Kyber.Compress.decompress_pre 10uy coefficient1);
+          assume (Libcrux.Kem.Kyber.Compress.decompress_pre 10uy coefficient2);
+          assume (Libcrux.Kem.Kyber.Compress.decompress_pre 10uy coefficient3);
+          assume (Libcrux.Kem.Kyber.Compress.decompress_pre 10uy coefficient4);
           let coefficient1 = (Libcrux.Kem.Kyber.Compress.decompress_ciphertext_coefficient 10uy coefficient1
                            <:
                            i32) in
-          assume (Libcrux.Kem.Kyber.Compress.decompress_pre 10uy coefficient2);
           let coefficient2 = (Libcrux.Kem.Kyber.Compress.decompress_ciphertext_coefficient 10uy coefficient2
                            <:
                            i32) in
-          assume (Libcrux.Kem.Kyber.Compress.decompress_pre 10uy coefficient3);
           let coefficient3 = (Libcrux.Kem.Kyber.Compress.decompress_ciphertext_coefficient 10uy coefficient3
                            <:
                            i32) in
-          assume (Libcrux.Kem.Kyber.Compress.decompress_pre 10uy coefficient4);
           let coefficient4 = (Libcrux.Kem.Kyber.Compress.decompress_ciphertext_coefficient 10uy coefficient4
                            <:
                            i32) in
-          // assume (v (sz 4 *! i) + 4 <= 256);
-          // assume (range (4 * v i) usize_inttype);
-          // assume (sz 4 *! i <. length (re.Libcrux.Kem.Kyber.Arithmetic.f_coefficients));
-          // let re:Libcrux.Kem.Kyber.Arithmetic.wfPolynomialRingElement =
-          //   {
-          //     re with
-          //     Libcrux.Kem.Kyber.Arithmetic.f_coefficients
-          //     =
-          //     Rust_primitives.Hax.Monomorphized_update_at.update_at_usize re
-          //         .Libcrux.Kem.Kyber.Arithmetic.f_coefficients
-          //       (sz 4 *! i <: usize)
-          //       coefficient1 
-          //   }
-          //   <:
-          //   Libcrux.Kem.Kyber.Arithmetic.wfPolynomialRingElement
-          // in
-          admit ();
-          // let re:Libcrux.Kem.Kyber.Arithmetic.wfPolynomialRingElement =
-          //   {
-          //     re with
-          //     Libcrux.Kem.Kyber.Arithmetic.f_coefficients
-          //     =
-          //     Rust_primitives.Hax.Monomorphized_update_at.update_at_usize re
-          //         .Libcrux.Kem.Kyber.Arithmetic.f_coefficients
-          //       ((sz 4 *! i <: usize) +! sz 1 <: usize)
-          //       coefficient2 
-          //   }
-          //   <:
-          //   Libcrux.Kem.Kyber.Arithmetic.wfPolynomialRingElement
-          // in
-          // let re:Libcrux.Kem.Kyber.Arithmetic.wfPolynomialRingElement =
-          //   {
-          //     re with
-          //     Libcrux.Kem.Kyber.Arithmetic.f_coefficients
-          //     =
-          //     Rust_primitives.Hax.Monomorphized_update_at.update_at_usize re
-          //         .Libcrux.Kem.Kyber.Arithmetic.f_coefficients
-          //       ((sz 4 *! i <: usize) +! sz 2 <: usize)
-          //       coefficient3
-          //   }
-          //   <:
-          //   Libcrux.Kem.Kyber.Arithmetic.wfPolynomialRingElement
-          // in
-          // let re:Libcrux.Kem.Kyber.Arithmetic.wfPolynomialRingElement =
-          //   {
-          //     re with
-          //     Libcrux.Kem.Kyber.Arithmetic.f_coefficients
-          //     =
-          //     Rust_primitives.Hax.Monomorphized_update_at.update_at_usize re
-          //         .Libcrux.Kem.Kyber.Arithmetic.f_coefficients
-          //       ((sz 4 *! i <: usize) +! sz 3 <: usize)
-          //       coefficient4
-          //   }
-          //   <:
-          //   Libcrux.Kem.Kyber.Arithmetic.wfPolynomialRingElement
-          // in
+          assert_spinoff (v i < 64 ==> 4 * v i + 4 <= 256);
+          assert_spinoff (v i < 64 ==> range (v (sz 4) * v i) usize_inttype);
+          let re:Libcrux.Kem.Kyber.Arithmetic.wfPolynomialRingElement =
+            {
+              re with
+              Libcrux.Kem.Kyber.Arithmetic.f_coefficients
+              =
+              Rust_primitives.Hax.Monomorphized_update_at.update_at_usize re
+                  .Libcrux.Kem.Kyber.Arithmetic.f_coefficients
+                (sz 4 *! i <: usize)
+                coefficient1 
+            }
+            <:
+            Libcrux.Kem.Kyber.Arithmetic.wfPolynomialRingElement
+          in
+          let re:Libcrux.Kem.Kyber.Arithmetic.wfPolynomialRingElement =
+            {
+              re with
+              Libcrux.Kem.Kyber.Arithmetic.f_coefficients
+              =
+              Rust_primitives.Hax.Monomorphized_update_at.update_at_usize re
+                  .Libcrux.Kem.Kyber.Arithmetic.f_coefficients
+                ((sz 4 *! i <: usize) +! sz 1 <: usize)
+                coefficient2 
+            }
+            <:
+            Libcrux.Kem.Kyber.Arithmetic.wfPolynomialRingElement
+          in
+          let re:Libcrux.Kem.Kyber.Arithmetic.wfPolynomialRingElement =
+            {
+              re with
+              Libcrux.Kem.Kyber.Arithmetic.f_coefficients
+              =
+              Rust_primitives.Hax.Monomorphized_update_at.update_at_usize re
+                  .Libcrux.Kem.Kyber.Arithmetic.f_coefficients
+                ((sz 4 *! i <: usize) +! sz 2 <: usize)
+                coefficient3
+            }
+            <:
+            Libcrux.Kem.Kyber.Arithmetic.wfPolynomialRingElement
+          in
+          let re:Libcrux.Kem.Kyber.Arithmetic.wfPolynomialRingElement =
+            {
+              re with
+              Libcrux.Kem.Kyber.Arithmetic.f_coefficients
+              =
+              Rust_primitives.Hax.Monomorphized_update_at.update_at_usize re
+                  .Libcrux.Kem.Kyber.Arithmetic.f_coefficients
+                ((sz 4 *! i <: usize) +! sz 3 <: usize)
+                coefficient4
+            }
+            <:
+            Libcrux.Kem.Kyber.Arithmetic.wfPolynomialRingElement
+          in
           re)
   in
-  admit ();
   re
 #pop-options
 
-let deserialize_then_decompress_11_ (serialized: t_Slice u8)
+#push-options "--z3rlimit 80"
+let deserialize_then_decompress_11_ serialized
     : Libcrux.Kem.Kyber.Arithmetic.wfPolynomialRingElement =
   let _:Prims.unit = () <: Prims.unit in
   let re:Libcrux.Kem.Kyber.Arithmetic.wfPolynomialRingElement =
@@ -648,19 +715,18 @@ let deserialize_then_decompress_11_ (serialized: t_Slice u8)
       (fun re temp_1_ ->
           let re:Libcrux.Kem.Kyber.Arithmetic.wfPolynomialRingElement = re in
           let i, bytes:(usize & t_Array u8 (sz 11)) = temp_1_ in
-          assume (length bytes == sz 11);
-          assume (v i * 8 + 8 <= 256);
-          let byte1:i32 = cast (bytes.[ sz 0 ] <: u8) <: i32 in
-          let byte2:i32 = cast (bytes.[ sz 1 ] <: u8) <: i32 in
-          let byte3:i32 = cast (bytes.[ sz 2 ] <: u8) <: i32 in
-          let byte4:i32 = cast (bytes.[ sz 3 ] <: u8) <: i32 in
-          let byte5:i32 = cast (bytes.[ sz 4 ] <: u8) <: i32 in
-          let byte6:i32 = cast (bytes.[ sz 5 ] <: u8) <: i32 in
-          let byte7:i32 = cast (bytes.[ sz 6 ] <: u8) <: i32 in
-          let byte8:i32 = cast (bytes.[ sz 7 ] <: u8) <: i32 in
-          let byte9:i32 = cast (bytes.[ sz 8 ] <: u8) <: i32 in
-          let byte10:i32 = cast (bytes.[ sz 9 ] <: u8) <: i32 in
-          let byte11:i32 = cast (bytes.[ sz 10 ] <: u8) <: i32 in
+          assert (v i < 32);
+          let byte1: int_t_d i32_inttype 8 = cast (bytes.[ sz 0 ] <: u8) <: i32 in
+          let byte2: int_t_d i32_inttype 8 = cast (bytes.[ sz 1 ] <: u8) <: i32 in
+          let byte3: int_t_d i32_inttype 8 = cast (bytes.[ sz 2 ] <: u8) <: i32 in
+          let byte4: int_t_d i32_inttype 8 = cast (bytes.[ sz 3 ] <: u8) <: i32 in
+          let byte5: int_t_d i32_inttype 8 = cast (bytes.[ sz 4 ] <: u8) <: i32 in
+          let byte6: int_t_d i32_inttype 8 = cast (bytes.[ sz 5 ] <: u8) <: i32 in
+          let byte7: int_t_d i32_inttype 8 = cast (bytes.[ sz 6 ] <: u8) <: i32 in
+          let byte8: int_t_d i32_inttype 8 = cast (bytes.[ sz 7 ] <: u8) <: i32 in
+          let byte9: int_t_d i32_inttype 8 = cast (bytes.[ sz 8 ] <: u8) <: i32 in
+          let byte10: int_t_d i32_inttype 8 = cast (bytes.[ sz 9 ] <: u8) <: i32 in
+          let byte11: int_t_d i32_inttype 8 = cast (bytes.[ sz 10 ] <: u8) <: i32 in
           let
           coefficient1,
           coefficient2,
@@ -689,7 +755,8 @@ let deserialize_then_decompress_11_ (serialized: t_Slice u8)
           let coefficient6 = Libcrux.Kem.Kyber.Compress.decompress_ciphertext_coefficient 11uy coefficient6 in
           let coefficient7 = Libcrux.Kem.Kyber.Compress.decompress_ciphertext_coefficient 11uy coefficient7 in
           let coefficient8 = Libcrux.Kem.Kyber.Compress.decompress_ciphertext_coefficient 11uy coefficient8 in
-          admit();
+          assert_spinoff (8 * v i + 8 <= 256);
+          assert_spinoff (range (v (sz 8) * v i) usize_inttype);
           let re:Libcrux.Kem.Kyber.Arithmetic.wfPolynomialRingElement =
             {
               re with
@@ -797,10 +864,10 @@ let deserialize_then_decompress_11_ (serialized: t_Slice u8)
           re)
   in
   re
+#pop-options
 
 #push-options "--z3rlimit 100"
-let deserialize_then_decompress_4_ (serialized: t_Slice u8)
-    : Libcrux.Kem.Kyber.Arithmetic.wfPolynomialRingElement =
+let deserialize_then_decompress_4_ serialized =
   let _:Prims.unit = () <: Prims.unit in
   let re:Libcrux.Kem.Kyber.Arithmetic.wfPolynomialRingElement =
     Libcrux.Kem.Kyber.Arithmetic.cast_poly_b Libcrux.Kem.Kyber.Arithmetic.impl__PolynomialRingElement__ZERO
@@ -812,11 +879,11 @@ let deserialize_then_decompress_4_ (serialized: t_Slice u8)
       (fun re temp_1_ ->
           let re:Libcrux.Kem.Kyber.Arithmetic.wfPolynomialRingElement = re in
           let i, byte:(usize & u8) = temp_1_ in
-          assume (v i * 2 + 2 <= 256);
           let coefficient1, coefficient2:(i32 & i32) = decompress_coefficients_4_ byte in
           assume (Libcrux.Kem.Kyber.Compress.decompress_pre 4uy coefficient1);
           assume (Libcrux.Kem.Kyber.Compress.decompress_pre 4uy coefficient2);
-          admit ();
+          assert_spinoff (v i < 128 ==> 2 * v i + 1 < 256);
+          assert_spinoff (v i < 128 ==> range (v (sz 2) * v i) usize_inttype);
           let re:Libcrux.Kem.Kyber.Arithmetic.wfPolynomialRingElement =
             {
               re with
@@ -847,15 +914,13 @@ let deserialize_then_decompress_4_ (serialized: t_Slice u8)
             <:
             Libcrux.Kem.Kyber.Arithmetic.wfPolynomialRingElement
           in
-          admit ();
           re)
   in
   re
 #pop-options
 
-let deserialize_then_decompress_5_ (serialized: t_Slice u8)
-    : Libcrux.Kem.Kyber.Arithmetic.wfPolynomialRingElement =
-   admit ();
+#push-options "--z3rlimit 150"
+let deserialize_then_decompress_5_ serialized =
   let _:Prims.unit = () <: Prims.unit in
   let re:Libcrux.Kem.Kyber.Arithmetic.wfPolynomialRingElement =
     Libcrux.Kem.Kyber.Arithmetic.cast_poly_b Libcrux.Kem.Kyber.Arithmetic.impl__PolynomialRingElement__ZERO
@@ -866,14 +931,14 @@ let deserialize_then_decompress_5_ (serialized: t_Slice u8)
       re
       (fun re temp_1_ ->
           let re:Libcrux.Kem.Kyber.Arithmetic.wfPolynomialRingElement = re in
-          let i, bytes:(usize & t_Array u8 (sz 5)) = temp_1_ in
-          assume (length bytes = sz 5);
-          assume (v i * 8 + 8 <= 256);
-          let byte1:i32 = cast (bytes.[ sz 0 ] <: u8) <: i32 in
-          let byte2:i32 = cast (bytes.[ sz 1 ] <: u8) <: i32 in
-          let byte3:i32 = cast (bytes.[ sz 2 ] <: u8) <: i32 in
-          let byte4:i32 = cast (bytes.[ sz 3 ] <: u8) <: i32 in
-          let byte5:i32 = cast (bytes.[ sz 4 ] <: u8) <: i32 in
+          let i, bytes:(usize & t_Array (int_t_d u8_inttype 5) (sz 5)) = temp_1_ in
+          assert (v i < 32);
+          let byte1 = cast (bytes.[ sz 0 ] <: u8) <: i32 in
+          let byte2 = cast (bytes.[ sz 1 ] <: u8) <: i32 in
+          let byte3 = cast (bytes.[ sz 2 ] <: u8) <: i32 in
+          let byte4 = cast (bytes.[ sz 3 ] <: u8) <: i32 in
+          let byte5 = cast (bytes.[ sz 4 ] <: u8) <: i32 in
+          assert (bounded byte1 5 /\ bounded byte2 5 /\ bounded byte3 5 /\ bounded byte4 5 /\ bounded byte5 5);
           let
           coefficient1,
           coefficient2,
@@ -902,6 +967,13 @@ let deserialize_then_decompress_5_ (serialized: t_Slice u8)
           let coefficient6 = Libcrux.Kem.Kyber.Compress.decompress_ciphertext_coefficient 5uy coefficient6 in
           let coefficient7 = Libcrux.Kem.Kyber.Compress.decompress_ciphertext_coefficient 5uy coefficient7 in
           let coefficient8 = Libcrux.Kem.Kyber.Compress.decompress_ciphertext_coefficient 5uy coefficient8 in
+          // assert (Seq.length serialized == 160);
+          // // assert_norm (160 / 5 == 32);
+          // assert_spinoff (v i < Seq.length serialized);
+          // assert (v i < 32);
+          assert_spinoff (v i < 32 ==> 8 * v i + 8 <= 256);
+          mul_in_range 8 (v i);
+          assert_spinoff (v i < 32 ==> range (v (sz 8) * v i) usize_inttype);
           let re:Libcrux.Kem.Kyber.Arithmetic.wfPolynomialRingElement =
             {
               re with
@@ -954,7 +1026,6 @@ let deserialize_then_decompress_5_ (serialized: t_Slice u8)
             <:
             Libcrux.Kem.Kyber.Arithmetic.wfPolynomialRingElement
           in
-          admit();
           let re:Libcrux.Kem.Kyber.Arithmetic.wfPolynomialRingElement =
             {
               re with
@@ -1010,9 +1081,11 @@ let deserialize_then_decompress_5_ (serialized: t_Slice u8)
           re)
   in
   re
+#pop-options
 
+// TODO
+#push-options "--z3rlimit 60"
 let deserialize_then_decompress_message (serialized: t_Array u8 (sz 32)) =
-  admit ();
   let re:Libcrux.Kem.Kyber.Arithmetic.wfPolynomialRingElement =
    Libcrux.Kem.Kyber.Arithmetic.cast_poly_b Libcrux.Kem.Kyber.Arithmetic.impl__PolynomialRingElement__ZERO
   in
@@ -1023,7 +1096,6 @@ let deserialize_then_decompress_message (serialized: t_Array u8 (sz 32)) =
       (fun re temp_1_ ->
           let re:Libcrux.Kem.Kyber.Arithmetic.wfPolynomialRingElement = re in
           let i, byte:(usize & u8) = temp_1_ in
-          assume (i <. sz 32);
           Core.Iter.Traits.Iterator.f_fold (Core.Iter.Traits.Collect.f_into_iter ({
                     Core.Ops.Range.f_start = sz 0;
                     Core.Ops.Range.f_end = sz 8
@@ -1037,7 +1109,7 @@ let deserialize_then_decompress_message (serialized: t_Array u8 (sz 32)) =
                 let re:Libcrux.Kem.Kyber.Arithmetic.wfPolynomialRingElement = re in
                 let j:usize = j in
                 let coefficient_compressed:i32 = cast ((byte >>! j <: u8) &. 1uy <: u8) <: i32 in
-                assume (coefficient_compressed =. 0l || coefficient_compressed =. 1l);
+                lemma_get_bit_bounded' coefficient_compressed 1;
                 let re:Libcrux.Kem.Kyber.Arithmetic.wfPolynomialRingElement =
                   {
                     re with
@@ -1060,11 +1132,12 @@ let deserialize_then_decompress_message (serialized: t_Array u8 (sz 32)) =
   in
   admit(); //P-F
   re
+#pop-options
 
 let deserialize_then_decompress_ring_element_u v_COMPRESSION_FACTOR serialized = 
   let _:Prims.unit = () <: Prims.unit in
   mk_int_equiv_lemma #usize_inttype (v v_COMPRESSION_FACTOR);
-  admit ();
+  assert (v (cast (v_COMPRESSION_FACTOR <: usize) <: u32) == 10 \/ v (cast (v_COMPRESSION_FACTOR <: usize) <: u32) == 11);
   match cast (v_COMPRESSION_FACTOR <: usize) <: u32 with
   | 10ul -> deserialize_then_decompress_10_ serialized
   | 11ul -> deserialize_then_decompress_11_ serialized
@@ -1076,8 +1149,8 @@ let deserialize_then_decompress_ring_element_u v_COMPRESSION_FACTOR serialized =
 
 let deserialize_then_decompress_ring_element_v v_COMPRESSION_FACTOR serialized =
   let _:Prims.unit = () <: Prims.unit in
-  assume (v v_COMPRESSION_FACTOR == 4 \/ v v_COMPRESSION_FACTOR == 5);
   mk_int_equiv_lemma #u32_inttype (v v_COMPRESSION_FACTOR);
+  assert (v (cast (v_COMPRESSION_FACTOR <: usize) <: u32) == 4 \/ v (cast (v_COMPRESSION_FACTOR <: usize) <: u32) == 5);
   let res = 
   match cast (v_COMPRESSION_FACTOR <: usize) <: u32 with
   | 4ul -> deserialize_then_decompress_4_ serialized
@@ -1091,6 +1164,7 @@ let deserialize_then_decompress_ring_element_v v_COMPRESSION_FACTOR serialized =
   admit(); //P-F
   res
 
+#push-options "--z3rlimit 100"
 let deserialize_to_uncompressed_ring_element (serialized: t_Slice u8) = 
   let _:Prims.unit = () <: Prims.unit in
   let re:Libcrux.Kem.Kyber.Arithmetic.wfPolynomialRingElement =
@@ -1103,12 +1177,14 @@ let deserialize_to_uncompressed_ring_element (serialized: t_Slice u8) =
       re
       (fun re temp_1_ ->
           let re:Libcrux.Kem.Kyber.Arithmetic.wfPolynomialRingElement = re in
-          let i, bytes:(usize & t_Array u8 (sz 3)) = admit (); temp_1_ in
-          assume (length bytes = sz 3);
-          assume (v i * 2 + 2 <= 256);
-          let byte1:i32 = cast (bytes.[ sz 0 ] <: u8) <: i32 in
-          let byte2:i32 = cast (bytes.[ sz 1 ] <: u8) <: i32 in
-          let byte3:i32 = cast (bytes.[ sz 2 ] <: u8) <: i32 in
+          let i, bytes:(usize & t_Array u8 (sz 3)) = temp_1_ in
+          let byte1:int_t_d i32_inttype 8 = cast (bytes.[ sz 0 ] <: u8) <: i32 in
+          let byte2:int_t_d i32_inttype 8 = cast (bytes.[ sz 1 ] <: u8) <: i32 in
+          let byte3:int_t_d i32_inttype 8 = cast (bytes.[ sz 2 ] <: u8) <: i32 in
+          let coef1 = (((byte2 &. 15l <: i32) <<! 8l <: i32) |. (byte1 &. 255l <: i32) <: i32) in
+          let coef2 = ((byte3 <<! 4l <: i32) |. ((byte2 >>! 4l <: i32) &. 15l <: i32) <: i32) in
+          lemma_get_bit_bounded' coef1 11;
+          lemma_get_bit_bounded' coef2 11;
           let re:Libcrux.Kem.Kyber.Arithmetic.wfPolynomialRingElement =
             {
               re with
@@ -1117,7 +1193,7 @@ let deserialize_to_uncompressed_ring_element (serialized: t_Slice u8) =
               Rust_primitives.Hax.Monomorphized_update_at.update_at_usize re
                   .Libcrux.Kem.Kyber.Arithmetic.f_coefficients
                 (sz 2 *! i <: usize)
-                (((byte2 &. 15l <: i32) <<! 8l <: i32) |. (byte1 &. 255l <: i32) <: i32)
+                coef1
             }
             <:
             Libcrux.Kem.Kyber.Arithmetic.wfPolynomialRingElement
@@ -1130,7 +1206,7 @@ let deserialize_to_uncompressed_ring_element (serialized: t_Slice u8) =
               Rust_primitives.Hax.Monomorphized_update_at.update_at_usize re
                   .Libcrux.Kem.Kyber.Arithmetic.f_coefficients
                 ((sz 2 *! i <: usize) +! sz 1 <: usize)
-                ((byte3 <<! 4l <: i32) |. ((byte2 >>! 4l <: i32) &. 15l <: i32) <: i32)
+                coef2
             }
             <:
             Libcrux.Kem.Kyber.Arithmetic.wfPolynomialRingElement
@@ -1138,11 +1214,11 @@ let deserialize_to_uncompressed_ring_element (serialized: t_Slice u8) =
           re)
   in
   re
+#pop-options
 
 #push-options "--z3rlimit 100"
 let serialize_uncompressed_ring_element (re: Libcrux.Kem.Kyber.Arithmetic.wfPolynomialRingElement) =
   let serialized:t_Array u8 (sz 384) = Rust_primitives.Hax.repeat 0uy (sz 384) in
-  admit();
   let serialized:t_Array u8 (sz 384) =
     Rust_primitives.Iterators.foldi_chunks_exact #_ #_ #(fun _ _ -> True)
       (Rust_primitives.unsize re.Libcrux.Kem.Kyber.Arithmetic.f_coefficients)
@@ -1150,21 +1226,19 @@ let serialize_uncompressed_ring_element (re: Libcrux.Kem.Kyber.Arithmetic.wfPoly
       serialized
       (fun serialized temp_1_ ->
           let serialized:t_Array u8 (sz 384) = serialized in
-          let i, coefficients:(usize & t_Array i32 (sz 2)) = temp_1_ in
-//          assume (Libcrux.Kem.Kyber.Arithmetic.to_unsigned_representative_pre coefficients.[ sz 0 ]);
+          let i, coefficients:(usize & t_Array (Libcrux.Kem.Kyber.Arithmetic.i32_b (v Libcrux.Kem.Kyber.Constants.v_FIELD_MODULUS - 1)) (sz 2)) = temp_1_ in
+          assert (v i < 128);
           let coefficient1:u16 =
             Libcrux.Kem.Kyber.Arithmetic.to_unsigned_representative (coefficients.[ sz 0 ] <: i32)
           in
-//          assume (Libcrux.Kem.Kyber.Arithmetic.to_unsigned_representative_pre coefficients.[ sz 1 ]);
           let coefficient2:u16 =
             Libcrux.Kem.Kyber.Arithmetic.to_unsigned_representative (coefficients.[ sz 1 ] <: i32)
           in
           let coef1, coef2, coef3:(u8 & u8 & u8) =
-           (*assume (int_t_has_bit_num coefficient1 12);
-            assume (int_t_has_bit_num coefficient2 12); *)
             compress_coefficients_3_ coefficient1 coefficient2
           in
-          assume (3 * v i + 3 <= 384);
+          assert_spinoff (3 * v i + 3 <= 384);
+          assert_spinoff (range (v (sz 3) * v i) usize_inttype);
           let serialized:t_Array u8 (sz 384) =
             Rust_primitives.Hax.Monomorphized_update_at.update_at_usize serialized
               (sz 3 *! i <: usize)
