proofs/fstar/extraction-edited/Libcrux.Kem.Kyber.Serialize.PartB.fsti
@@ -5,22 +5,22 @@ open FStar.Mul
 open MkSeq
 
 val compress_then_serialize_10_
-      (v_OUT_LEN: usize)
+      (v_OUT_LEN: usize {v v_OUT_LEN >= 320})
       (re: Libcrux.Kem.Kyber.Arithmetic.wfPolynomialRingElement)
     : Prims.Pure (t_Array u8 v_OUT_LEN) Prims.l_True (fun _ -> Prims.l_True)
 
 val compress_then_serialize_11_
-      (v_OUT_LEN: usize)
+      (v_OUT_LEN: usize {v v_OUT_LEN >= 352})
       (re: Libcrux.Kem.Kyber.Arithmetic.wfPolynomialRingElement)
     : Prims.Pure (t_Array u8 v_OUT_LEN) Prims.l_True (fun _ -> Prims.l_True)
 
 val compress_then_serialize_4_
-      (v_OUT_LEN: usize)
+      (v_OUT_LEN: usize {v v_OUT_LEN >= 256})
       (re: Libcrux.Kem.Kyber.Arithmetic.wfPolynomialRingElement)
     : Prims.Pure (t_Array u8 v_OUT_LEN) Prims.l_True (fun _ -> Prims.l_True)
 
 val compress_then_serialize_5_
-      (v_OUT_LEN: usize)
+      (v_OUT_LEN: usize {v v_OUT_LEN >= 160})
       (re: Libcrux.Kem.Kyber.Arithmetic.wfPolynomialRingElement)
     : Prims.Pure (t_Array u8 v_OUT_LEN) Prims.l_True (fun _ -> Prims.l_True)
 
@@ -30,8 +30,15 @@ val compress_then_serialize_message (re: Libcrux.Kem.Kyber.Arithmetic.wfPolynomi
       (ensures (fun res ->
         res == Spec.Kyber.compress_then_encode_message (Libcrux.Kem.Kyber.Arithmetic.to_spec_poly_b re)))
 
-val compress_then_serialize_ring_element_u (#p:Spec.Kyber.params)
-      (v_COMPRESSION_FACTOR v_OUT_LEN: usize)
+val compress_then_serialize_ring_element_u
+      (#p:Spec.Kyber.params)
+      (v_COMPRESSION_FACTOR: usize)
+      (v_OUT_LEN: usize {
+        match v v_COMPRESSION_FACTOR with
+        | 10 -> v v_OUT_LEN >= 320
+        | 11 -> v v_OUT_LEN >= 352
+        | _ -> False
+      })
       (re: Libcrux.Kem.Kyber.Arithmetic.wfPolynomialRingElement)
     : Pure (t_Array u8 v_OUT_LEN)
       (requires (v_COMPRESSION_FACTOR = sz 10 || v_COMPRESSION_FACTOR = sz 11) /\
@@ -39,7 +46,13 @@ val compress_then_serialize_ring_element_u (#p:Spec.Kyber.params)
       (ensures (fun _ -> True)) 
       
 val compress_then_serialize_ring_element_v (#p:Spec.Kyber.params)
-      (v_COMPRESSION_FACTOR v_OUT_LEN: usize)
+      (v_COMPRESSION_FACTOR: usize)
+      (v_OUT_LEN: usize {
+        match v v_COMPRESSION_FACTOR with
+        | 4 -> v v_OUT_LEN >= 256
+        | 5 -> v v_OUT_LEN >= 160
+        | _ -> False
+      })
       (re: Libcrux.Kem.Kyber.Arithmetic.wfPolynomialRingElement)
     : Pure (t_Array u8 v_OUT_LEN)
       (requires (v_COMPRESSION_FACTOR = sz 4 || v_COMPRESSION_FACTOR = sz 5) /\
@@ -49,22 +62,23 @@ val compress_then_serialize_ring_element_v (#p:Spec.Kyber.params)
         Spec.Kyber.compress_then_encode_v p 
           (Libcrux.Kem.Kyber.Arithmetic.to_spec_poly_b re)))
 
-val deserialize_then_decompress_10_ (serialized: t_Slice u8)
+val deserialize_then_decompress_10_ (serialized: t_Slice u8 {Seq.length serialized == 320})
     : Prims.Pure Libcrux.Kem.Kyber.Arithmetic.wfPolynomialRingElement
       Prims.l_True
       (fun _ -> Prims.l_True)
 
-val deserialize_then_decompress_11_ (serialized: t_Slice u8)
+val deserialize_then_decompress_11_ (serialized: t_Slice u8 {Seq.length serialized == 352})
     : Prims.Pure Libcrux.Kem.Kyber.Arithmetic.wfPolynomialRingElement
       Prims.l_True
       (fun _ -> Prims.l_True)
 
-val deserialize_then_decompress_4_ (serialized: t_Slice u8)
+val deserialize_then_decompress_4_ (serialized: t_Slice u8 {Seq.length serialized == 128})
     : Prims.Pure Libcrux.Kem.Kyber.Arithmetic.wfPolynomialRingElement
       Prims.l_True
       (fun _ -> Prims.l_True)
 
-val deserialize_then_decompress_5_ (serialized: t_Slice u8)
+val deserialize_then_decompress_5_ 
+  (serialized: t_Slice (int_t_d u8_inttype 5) {Seq.length serialized == 160})
     : Prims.Pure Libcrux.Kem.Kyber.Arithmetic.wfPolynomialRingElement
       Prims.l_True
       (fun _ -> Prims.l_True)
@@ -78,21 +92,27 @@ val deserialize_then_decompress_message (serialized: t_Array u8 (sz 32))
 
 val deserialize_then_decompress_ring_element_u
       (v_COMPRESSION_FACTOR: usize)
-      (serialized: t_Slice u8)
+      (serialized: t_Slice u8 {
+        match v v_COMPRESSION_FACTOR with
+        | 10 -> Seq.length serialized == 320
+        | 11 -> Seq.length serialized == 352
+        | _ -> False
+      })
     : Pure (Libcrux.Kem.Kyber.Arithmetic.wfPolynomialRingElement)
       (requires v_COMPRESSION_FACTOR = sz 10 || v_COMPRESSION_FACTOR = sz 11)
       (ensures fun _ -> True)
 
 val deserialize_then_decompress_ring_element_v (#p:Spec.Kyber.params)
-      (v_COMPRESSION_FACTOR: usize)
-      (serialized: t_Slice u8)
+      (v_COMPRESSION_FACTOR: usize {v v_COMPRESSION_FACTOR == 4 \/ v v_COMPRESSION_FACTOR == 5})
+      (serialized: t_Slice (if v v_COMPRESSION_FACTOR = 4 then u8 else int_t_d u8_inttype 5))
     : Pure (Libcrux.Kem.Kyber.Arithmetic.wfPolynomialRingElement)
       (requires (p.v_VECTOR_V_COMPRESSION_FACTOR == v_COMPRESSION_FACTOR /\
                  length serialized == Spec.Kyber.v_C2_SIZE p))
       (ensures fun res ->
-       Libcrux.Kem.Kyber.Arithmetic.to_spec_poly_b res ==
-       Spec.Kyber.decode_then_decompress_v p serialized)
-
+        True
+       // Libcrux.Kem.Kyber.Arithmetic.to_spec_poly_b res ==
+       // Spec.Kyber.decode_then_decompress_v p serialized
+       )
 
 val deserialize_to_uncompressed_ring_element (serialized: t_Slice u8)
     : Pure (Libcrux.Kem.Kyber.Arithmetic.wfPolynomialRingElement)
